The crowdfunding example

ExampleContracts.v
@@ -1,170 +1,319 @@
 Require Import String.
-Require Import Ast.
-Require Import EvalE.
+Require Import Ast EvalE CustomTactics.
 Require Import List.
+Require Import PeanoNat.
 Import ListNotations.
 From Template Require Import All.
-
 
 Import MonadNotation.
 Import BaseTypes.
 Import StdLib.
 Open Scope list.
-(* Example by Jakob *)
-(* Definition receive *)
-(*            (chain : PackedChain) *)
-(*            (ctx : ContractCallContext) *)
-(*            (state : State) *)
-(*            (msg : option Msg) : option (State * list ActionBody) := *)
-(*   match msg with *)
-(*   | Some msg_payme => *)
-(*     let sender := ctx_from ctx in *)
-(*     let me := ctx_contract_address ctx in *)
-(*     do amount <- FMap.find sender (money_owed state); *)
-(*       Some (state, *)
-(*             [act_transfer sender amount; *)
-(*              act_call me 0 (msg_continuation1 (build_continuation1 sender amount))]) *)
-(*   | Some (msg_continuation1 (build_continuation1 sender amount)) => *)
-(*     Some (state<|money_owed ::= FMap.add sender 0|>, []) *)
-(* end. *)
 
-Definition Address := nat.
-Definition Action := unit.
+Section Maps.
+  Open Scope nat.
 
-Record ctx := mkctx { _ctx_from : Address; _ctx_contract_address : Address}.
+  (* Our approximation for maps *)
+  Inductive addr_map : Set :=
+  | mnil | mcons : nat -> nat -> addr_map -> addr_map.
+
+  Inductive Maybe_map :=
+  | Just_map : nat -> Maybe_map | Nothing_map.
+
+  Definition Maybe := "Maybe_map".
+
+  Fixpoint lookup_map (m : addr_map) (key : nat) : Maybe_map :=
+    match m with
+    | mnil => Nothing_map
+    | mcons k v m' =>
+      if (Nat.eqb k key) then Just_map v else lookup_map m' key
+    end.
+
+  (* Ported from FMapWeaklist of StdLib *)
+  Function add_map (k : nat) (x : nat) (s : addr_map) : addr_map :=
+  match s with
+   | mnil => mcons k x mnil
+   | mcons k' y l => if Nat.eqb k k' then mcons k x l else mcons k' y (add_map k x l)
+  end.
+
+  Definition inmap_map k m := match lookup_map k m with
+                          | Just_map _ => true
+                          | Nothing => false
+                              end.
+
+  Lemma lookup_map_add k v m : lookup_map (add_map k v m) k = Just_map v.
+  Proof.
+    induction m.
+    + simpl. now rewrite PeanoNat.Nat.eqb_refl.
+    + simpl. destruct (k =? n) eqn:Heq.
+      * simpl. now rewrite PeanoNat.Nat.eqb_refl.
+      * simpl. rewrite Nat.eqb_sym. now rewrite Heq.
+  Qed.
+
+End Maps.
+
+Notation "a ∈ m" := (inmap_map a m = true) (at level 50).
+
+Fixpoint mkNames (ns : list string) (postfix : string) :=
+  match ns with
+  | [] => tmPrint "Done."
+  | n :: ns' => n' <- tmEval all (n ++ postfix)%string ;;
+                  str <- tmQuote n';;
+                  tmMkDefinition n str;;
+                  mkNames ns' postfix
+  end.
+
+Definition Map := "addr_map".
+
+Notation "'mfind' a b" :=  [| {eConst "lookup_map"} {a} {b} |]
+        (in custom expr at level 0,
+            a custom expr at level 1,
+            b custom expr at level 1).
+
+Notation "'madd' a b c" :=  [| {eConst "add_map"} {a} {b} {c} |]
+        (in custom expr at level 0,
+            a custom expr at level 1,
+            b custom expr at level 1,
+            c custom expr at level 1).
+
+Notation "'mem' a b" :=  [| {eConst "inmap_map"} {a} {b} |]
+        (in custom expr at level 0,
+            a custom expr at level 1,
+            b custom expr at level 1).
+
+Record ctx := mkctx { _ctx_from : nat;
+                      _ctx_contract_address : nat ;
+                      _amount : nat;
+                      _cur_time : nat}.
+
+
+(** Contract execution context  *)
+Definition ctx_from_name := "ExampleContracts._ctx_from".
+Definition Ctx := "ExampleContracts.ctx".
+Notation "'ctx_from' a" := [| {eConst ctx_from_name} {a} |]
+                             (in custom expr at level 0).
+Notation "'ctx_contract_address' a" :=
+  [| {eConst "ExampleContracts._ctx_contract_address"} {a} |]
+    (in custom expr at level 0).
+Notation "'amount' a" := [| {eConst "_amount"} {a} |]
+                             (in custom expr at level 0).
+Notation "'cur_time' a" := [| {eConst "_cur_time"} {a} |]
+                             (in custom expr at level 0).
+
 
 Module BalanceContract.
-  Record state := st { _balance : nat; _owner : Address }.
-  Inductive result :=
-  | res : state -> Action -> result
-  | error.
 
-  Inductive msg :=
-  | topup | withdraw.
+  Notation Address := Nat.
+  Definition Money := Nat.
 
+  (* Generating names for the data structures  *)
+  Run TemplateProgram
+      (mkNames ["State" ; "balance" ; "donations" ; "owner"; "deadline"; "goal";
+                "Result" ; "Res" ; "Error";
+                "Msg"; "Donate"; "GetFunds"; "Claim";
+                "Action"; "Transfer"; "Empty" ] "_coq").
 
-  Module ConstantMapping.
+  Import ListNotations.
 
-    Definition Address := "Coq.Init.Datatypes.nat".
-    Definition Money := "Coq.Init.Datatypes.nat".
-    Definition Result := "ExampleContracts.BalanceContract.result".
-    Definition Action := Unit.
+  Definition state_syn :=
+    [\ record State :=
+       { balance : Money ;
+         donations : Map;
+         owner : Money;
+         deadline : Nat;
+         goal : Money } \].
 
+  Make Inductive (trans_global_dec state_syn).
 
-    Definition Msg := "ExampleContracts.BalanceContract.msg".
-    Notation "'Topup'" := (pConstr "ExampleContracts.BalanceContract.Topup" []) (in custom pat at level 0).
-    Notation "'Withdraw'" := (pConstr "ExampleContracts.BalanceContract.Withdraw" []) ( in custom pat at level 0).
+  Definition action_syn :=
+    [\ data Action :=
+         Transfer : Address -> Money -> Action
+         | Empty : Action; \].
 
-    Definition State := "ExampleContracts.BalanceContract.state".
+  Make Inductive (trans_global_dec action_syn).
+
+  Definition result_syn :=
+    [\ data Result :=
+         Res : State -> Action -> Result
+       | Error : Result; \].
+
+  Make Inductive (trans_global_dec result_syn).
+
+  Definition msg_syn :=
+    [\ data Msg :=
+       Donate : Msg
+       | GetFunds : Msg
+       | Claim : Msg; \].
+
+  Make Inductive (trans_global_dec msg_syn).
+
+  Module Notations.
+
+    Notation "'Donate'" :=
+      (pConstr Donate []) (in custom pat at level 0).
+    Notation "'GetFunds'" :=
+      (pConstr GetFunds []) ( in custom pat at level 0).
+
+    Notation "'Claim'" :=
+      (pConstr Claim []) ( in custom pat at level 0).
+
+    Notation "'Just' x" :=
+      (pConstr "Just" [x]) (in custom pat at level 0,
+                               x constr at level 4).
+    Notation "'Nothing'" := (pConstr "Nothing" [])
+                              (in custom pat at level 0).
+
+    (* Notations for projections *)
     Notation "'balance' a" :=
-      [| {eConst "ExampleContracts.BalanceContract._balance"} {a} |]
+      [| {eConst balance} {a} |]
+        (in custom expr at level 0).
+    Notation "'donations' a" :=
+      [| {eConst donations} {a} |]
         (in custom expr at level 0).
     Notation "'owner' a" :=
-      [| {eConst "ExampleContracts.BalanceContract._owner"} {a} |]
+      [| {eConst owner} {a} |]
+        (in custom expr at level 0).
+    Notation "'deadline' a" :=
+      [| {eConst deadline} {a} |]
+        (in custom expr at level 0).
+    Notation "'goal' a" :=
+      [| {eConst goal} {a} |]
         (in custom expr at level 0).
 
     Notation "'Res' a b" :=
-      [| {eConstr Result "ExampleContracts.BalanceContract.res"} {a} {b} |]
+      [| {eConstr Result Res} {a} {b} |]
         (in custom expr at level 0,
             a custom expr at level 1,
             b custom expr at level 1).
 
-    Notation "'St' a b" :=
-      [| {eConstr State "ExampleContracts.BalanceContract.st"} {a} {b} |]
+    Notation "'Error'" := (eConstr Result Error)
+                        (in custom expr at level 0).
+
+    Notation "'mkState' a b" :=
+      [| {eConstr State "mkState_coq"} {a} {b} |]
         (in custom expr at level 0,
             a custom expr at level 1,
             b custom expr at level 1).
 
-    Definition Ctx := "ExampleContracts.ctx".
-    Notation "'ctx_from' a" := [| {eConst "ExampleContracts._ctx_from"} {a} |]
-                                 (in custom expr at level 0).
-    Notation "'ctx_contract_address' a" :=
-      [| {eConst "ExampleContracts._ctx_contract_address"} {a} |]
-        (in custom expr at level 0).
+    Notation "'Transfer' a b" :=
+      [| {eConstr Action Transfer} {a} {b} |]
+        (in custom expr at level 0,
+            a custom expr at level 1,
+            b custom expr at level 1).
 
-    Notation "'Error'" := (eConstr Result "ExampleContracts.BalanceContract.error")
+    Notation "'Empty'" := (eConstr Action Empty)
                         (in custom expr at level 0).
 
     (* New global context with the constants defined above (in addition to the ones defined in
        "StdLib") *)
+
+
     Definition Σ' :=
-    Σ ++ [gdInd Ctx [("ExampleContracts.mkctx", [tyInd Address; tyInd Address])];
-            gdInd "ExampleContracts.BalanceContract.state"
-                  [("ExampleContracts.BalanceContract.st", [tyInd Address; tyInd Money])];
-            gdInd "ExampleContracts.BalanceContract.result"
-                  [("ExampleContracts.BalanceContract.res", [tyInd State; tyInd Action]);
-                     ("ExampleContracts.BalanceContract.error", [])];
-            gdInd "ExampleContracts.BalanceContract.msg"
-                  [("ExampleContracts.BalanceContract.Topup",[]);
-                     ("ExampleContracts.BalanceContract.Withdraw",[])]].
+      Σ ++ [gdInd Ctx [("ExampleContracts.mkctx",
+                        [(nAnon,tyInd Address); (nAnon,tyInd Address)])] false;
+              gdInd Maybe [("Just", [(nAnon,tyInd Nat)]);
+                             ("Nothing", [])] false;
+            state_syn;
+            result_syn;
+            msg_syn;
+            action_syn].
 
 
-    End ConstantMapping.
+    End Notations.
 
-  Import ConstantMapping.
+  Import Notations.
 
-  Module Names.
-    (* Create a macro "define_names" using TemplateMonad *)
-    Definition c := "c".
-    Definition s := "s".
-    Definition e := "e".
-    Definition m := "m".
-    Definition amount := "amount".
-    Definition sender := "sender".
-    Definition own := "own".
-    Definition newstate := "newstate".
-    Definition cond := "cond".
-  End Names.
-
-  Import Names.
-
-  Notation "'if' cond 'then' b1 'else' b2" :=
-    (eCase (Bool,0) (tyInd Result) cond
+  Run TemplateProgram (mkNames ["c";"s";"e";"m";"v";
+                                "tx_amount"; "bal"; "sender"; "own";
+                                "accs"; "now";
+                                "newstate"; "newmap"; "cond"] "").
+  Notation "'if' cond 'then' b1 'else' b2 : ty" :=
+    (eCase (Bool,0) (tyInd ty) cond
            [(pConstr true_name [],b1);(pConstr false_name [],b2)])
       (in custom expr at level 0,
           cond custom expr at level 4,
+          ty constr at level 4,
           b1 custom expr at level 4,
           b2 custom expr at level 4).
 
   Definition contract : expr :=
-    [|
-     \c : Ctx ->
-          \s : State ->
-               \m : Msg ->
-                    case m : Msg return Result of
-                      | Withdraw ->
-                         let amount : Money := balance s in
-                         let sender : Address := ctx_from c in
-                         let own : Address := owner s in
-                         if own == sender then Res (St Z own) star else Error
-                      | Topup -> Error
+    [| \c : Ctx -> \s : State ->  \m : Msg ->
+         let bal : Money := balance s in
+         let now : Nat := cur_time c in
+         let tx_amount : Money := amount c in
+         let sender : Address := ctx_from c in
+         let own : Address := owner s in
+         let accs : Map := donations s in
+         case m : Msg return Result of
+            | GetFunds ->
+             if (own == sender) && (deadline s < now) && (goal s <= bal)  then
+               Res (mkState 0 accs own (deadline s) (goal s)) (Transfer bal sender)
+             else Error : Result
+           | Donate ->
+             (case (mfind accs sender) : Maybe return Result of
+               | Just v ->
+                 let newmap : Map := madd sender (v + tx_amount) accs in
+                 Res (mkState (tx_amount + bal) newmap own (deadline s) (goal s)) Empty
+               | Nothing ->
+                 let newmap : Map := madd sender tx_amount accs in
+                 Res (mkState (tx_amount + bal) newmap own (deadline s) (goal s)) Empty)
+           | Claim ->
+             if (deadline s < now) && (bal < goal s) then
+             (case (mfind accs sender) : Maybe return Result of
+              | Just v -> let newmap : Map := madd sender 0 accs in
+                  Res (mkState (bal-v) newmap own (deadline s) (goal s))
+                      (Transfer v sender)
+               | Nothing -> Error)
+              else Error : Result
     |].
 
   Make Definition entry :=
-      Eval compute in (expr_to_term Σ' (indexify nil contract)).
+    Eval compute in (expr_to_term Σ' (indexify nil contract)).
 
-  End BalanceContract.
+  Ltac split_andb := apply Bool.andb_true_iff;split.
 
-  Import BalanceContract.
-
-  Definition OwnerAddr := 123.
-  Definition CntrAddr := 321.
-
-  Definition CallCtx := mkctx OwnerAddr CntrAddr.
-
-  Lemma withdraw_correct (init_state final_state: state) msg out_tx :
+  Lemma get_money_back_guarantee (init_state final_state: State_coq)
+        CallCtx  msg sender out_tx v :
     (* pre-condition *)
-    init_state.(_balance) > 0 ->
-    init_state.(_owner) = OwnerAddr ->
-    msg = withdraw ->
+    sender = CallCtx.(_ctx_from) -> msg = Claim_coq -> (* a sender claims the money*)
+    init_state.(balance_coq) < init_state.(goal_coq)  (* the goal is not reached *)
+    -> lookup_map init_state.(donations_coq) sender = Just_map v (* the sender donated [v] *)
+    -> init_state.(deadline_coq) < CallCtx.(_cur_time) (* deadline have passed *)
 
-    entry CallCtx init_state msg = res final_state out_tx ->
+    -> entry CallCtx init_state msg = Res_coq final_state out_tx
 
-    (* post-condition (TODO: add a post-condition about the outgoing transaction) *)
-    final_state.(_balance) = 0.
+    (* post-condition *)
+    -> out_tx = Transfer_coq v sender (*the money are sent back *)
+      /\ lookup_map final_state.(donations_coq) sender = Just_map 0. (* balance of a sender put to zero *)
   Proof.
-    intros Hb Hi Hmsg Hcall. subst. simpl in *.
-    destruct (Nat.eqb (_owner init_state) OwnerAddr).
-    + inversion Hcall. easy.
-    + inversion Hcall.
+    intros Hmsg Hsender Hgoal Hlook Hdl Hcall.
+    subst;simpl in *.  rewrite <- Nat.ltb_lt in *.
+    (* direct rewriting with [Hlook] or [Hgoal] cannot unify terms
+       in Hcall for some reason, but destruct with uderscores works *)
+    destruct (_ && _)%bool;tryfalse.
+    destruct (lookup_map _ _);tryfalse; inversion Hlook;subst;clear Hlook.
+    split.
+    * inversion Hcall. reflexivity.
+    * inversion Hcall. subst. simpl.
+      now rewrite lookup_map_add.
   Qed.
+
+  (* Lemma GetFunds_correct (init_state final_state: State_coq) CallCtx *)
+  (*       msg out_tx OwnerAddr: *)
+  (*   CallCtx.(_ctx_from) = OwnerAddr -> *)
+  (*   (* pre-condition *) *)
+  (*   init_state.(balance_coq) > 0 -> *)
+  (*   init_state.(owner_coq) = OwnerAddr -> *)
+  (*   msg = GetFunds_coq -> *)
+
+  (*   entry CallCtx init_state msg = Res_coq final_state out_tx -> *)
+
+  (*   (* post-condition (TODO: add a post-condition about the outgoing transaction) *) *)
+  (*   final_state.(balance_coq) = 0. *)
+  (* Proof. *)
+  (*   intros Hown Hb Hi Hmsg Hcall. subst. simpl in *. *)
+  (*   rewrite <- Hi in Hcall. rewrite PeanoNat.Nat.eqb_refl in Hcall. *)
+  (*   inversion Hcall. easy. *)
+  (* Qed. *)
+
+End BalanceContract.
